Examples/BLS12/ExampleBLS12Solinas.v
@@ -7,7 +7,7 @@ Require Import Lia.
 Require Import Crypto.Arithmetic.Partition.
 Require Import Crypto.Arithmetic.UniformWeight.
 Require Import Crypto.Stringification.IR.
-Require Import QuadraticFieldExtensions.
+Require Import Theory.QuadraticFieldExtensions.
 Require Import Coqprime.elliptic.GZnZ.
 Require Import Field_theory.
 Require Import Ring_theory.
@@ -36,11 +36,22 @@ Local Open Scope list_scope.
 
 (*Definitions and notation*)
 
-Definition s := (2 ^ 127)%Z.
-Definition c := [(1, 1)].
-Definition p := Eval compute in (s - Associational.eval c).
-Definition w := uweight 64.
+Definition u := -0xd201000000010000.
+Definition p_of_u u := (((u - 1)^2 * (u^4 - u^2 + 1)) / 3) + u.
+Definition bitwidth := 64.
+Definition p := Eval compute in (p_of_u u).
+Definition w := uweight bitwidth.
 Notation "n 'zmod' p" := (mkznz p (n mod p) (modz p n)) (at level 90).
+Definition n := 6%nat.
+Definition r := 2^bitwidth.
+Definition r' := Eval compute in (val p (GZnZ.inv p (r zmod p))).
+Definition m' := Eval compute in (val r (GZnZ.inv r ((- p) zmod r))).
+
+Lemma r'_correct: (r * r') mod p = 1.
+Proof. auto. Qed.
+
+Lemma m'_correct: (p * m') mod r = (-1) mod r.
+Proof. auto. Qed.
 
 (*A few results on prime and base field.*)
 Lemma p_ge2: 2 < p.
@@ -63,11 +74,11 @@ Notation "x *Fp y" := (GZnZ.mul p x y) (at level 90).
 Notation "x -Fp y" := (GZnZ.sub p x y) (at level 100).
 
 (*Base field arithmetic, encoding and decoding*)
-Definition mulp x y := WordByWordMontgomery.mulmod 64 2 p 1 x y.
-Definition addp x y := WordByWordMontgomery.addmod 64 2 p x y.
-Definition subp x y := WordByWordMontgomery.submod 64 2 p x y.
-Definition tomont z := WordByWordMontgomery.encodemod 64 2 p 1 z.
-Definition evalp z := @WordByWordMontgomery.eval 64 2 (WordByWordMontgomery.from_montgomerymod 64 2 p 1 z).
+Definition mulp x y := WordByWordMontgomery.mulmod bitwidth n p m' x y.
+Definition addp x y := WordByWordMontgomery.addmod bitwidth n p x y.
+Definition subp x y := WordByWordMontgomery.submod bitwidth n p x y.
+Definition tomont z := WordByWordMontgomery.encodemod bitwidth n p m' z.
+Definition evalp z := @WordByWordMontgomery.eval bitwidth n (WordByWordMontgomery.from_montgomerymod bitwidth n p m' z).
 
 Local Notation "x '+p' y" := (addp x y) (at level 100).
 Local Notation "x *p y" := (mulp x y) (at level 90).
@@ -89,6 +100,28 @@ Definition subFp2 := fun x y => ((fst x) -p (fst y), (snd x) -p (snd y)).
 Definition tomontFp2:= fun x => (tomont (val p (fst x)), tomont (val p (snd x))).
 Definition evalFp2:= fun x => (evalp (fst x) zmod p, evalp (snd x) zmod p).
 
+(* 
+(*Testing*)
+Definition z11 := p - 2.
+Definition z12 := p / 2.
+Definition z21 := p - p /3.
+Definition z22 := p - p / 5.
+Definition m11 := tomont z11.
+Definition m12 := tomont z12.
+Definition m21 := tomont z21.
+Definition m22 := tomont z22.
+Definition prod := subFp2 (m11, m12) (m21, m22).
+
+Eval native_compute in (m11).
+Eval native_compute in (m12).
+Eval native_compute in (m21).
+Eval native_compute in (m22).
+
+Eval native_compute in (prod). *)
+
+
+
+
 
 (*A few auxillary results on field arithmetic*)
 Add Field fp : (FZpZ p p_prime).
@@ -103,33 +136,31 @@ Qed.
 Lemma karatsuba_correct: forall x1 x2 y1 y2, ((x1 +Fp x2) *Fp (y1 +Fp y2) -Fp x1 *Fp y1 -Fp x2 *Fp y2) = (x1 *Fp y2 +Fp x2 *Fp y1).
 Proof. intros; ring. Qed.
 
-Ltac lauto := auto with zarith; unfold p; lia.
 
 (*Proofs of validity (as in Crypto.Arithmetic.WordByWordMontgomery)*)
 
-
-(*Se på goal selection!!!*)
-Lemma tomont_valid: forall x, WordByWordMontgomery.valid 64 2 p (tomont (val p x)).
+Ltac lauto := auto with zarith; try unfold p; try unfold n; try unfold bitwidth; lia.
+Lemma tomont_valid: forall x, WordByWordMontgomery.valid bitwidth n p (tomont (val p x)).
 Proof.
-    intros; unfold tomont; pose proof WordByWordMontgomery.encodemod_correct 64 2 p (2^63) 1 as [_ H0].
-    1-6: lauto. apply H0; case x; intros; auto; simpl; rewrite inZnZ; apply Z_mod_lt; unfold p; lia.
+    intros; unfold tomont; pose proof WordByWordMontgomery.encodemod_correct bitwidth n p (r') m' as [_ H0].
+    1-6: lauto. apply H0; case x; intros; simpl; rewrite inZnZ; apply Z_mod_lt; unfold p; lia.
 Qed.
 
-Lemma add_valid: forall x y,WordByWordMontgomery.valid 64 2 p x -> WordByWordMontgomery.valid 64 2 p y -> WordByWordMontgomery.valid 64 2 p (x +p y).
+Lemma add_valid: forall x y,WordByWordMontgomery.valid bitwidth n p x -> WordByWordMontgomery.valid bitwidth n p y -> WordByWordMontgomery.valid bitwidth n p (x +p y).
 Proof.
-    intros; pose proof WordByWordMontgomery.addmod_correct 64 2 p (2^63) 1 as [_ H1].
+    intros; pose proof WordByWordMontgomery.addmod_correct bitwidth n p r' m' as [_ H1].
     1-6: lauto. apply H1; auto.
 Qed.
 
-Lemma sub_valid: forall x y,WordByWordMontgomery.valid 64 2 p x -> WordByWordMontgomery.valid 64 2 p y -> WordByWordMontgomery.valid 64 2 p (x -p y).
+Lemma sub_valid: forall x y,WordByWordMontgomery.valid bitwidth n p x -> WordByWordMontgomery.valid bitwidth n p y -> WordByWordMontgomery.valid bitwidth n p (x -p y).
 Proof.
-    intros; pose proof WordByWordMontgomery.submod_correct 64 2 p (2^63) 1 as [_ H1].
+    intros; pose proof WordByWordMontgomery.submod_correct bitwidth n p r' m' as [_ H1].
     1-6: lauto. apply H1; auto.
 Qed.
 
-Lemma mul_valid: forall x y,WordByWordMontgomery.valid 64 2 p x -> WordByWordMontgomery.valid 64 2 p y -> WordByWordMontgomery.valid 64 2 p (x *p y).
+Lemma mul_valid: forall x y,WordByWordMontgomery.valid bitwidth n p x -> WordByWordMontgomery.valid bitwidth n p y -> WordByWordMontgomery.valid bitwidth n p (x *p y).
 Proof.
-    intros; pose proof WordByWordMontgomery.mulmod_correct 64 2 p (2^63) 1 as [_ H1].
+    intros; pose proof WordByWordMontgomery.mulmod_correct bitwidth n p r' m' as [_ H1].
     1-6: lauto. apply H1; auto.
 Qed.
 
@@ -137,25 +168,25 @@ Qed.
 (*Correctness of evaluation wrt. operations and encoding*)
 Theorem eval_tomont_inv: forall val, 0 <= val < p -> evalp (tomont val) mod p = val.
 Proof.
-    intros val H; unfold evalp, tomont; rewrite WordByWordMontgomery.eval_encodemod with (r' := 2 ^ 63); try lauto.
+    intros val H; unfold evalp, tomont; rewrite WordByWordMontgomery.eval_encodemod with (r' := r'); try lauto.
 Qed.
 
-Lemma eval_sub: forall x y, WordByWordMontgomery.valid 64 2 p x -> WordByWordMontgomery.valid 64 2 p y -> (evalp (x -p y)) mod p = ( evalp x - evalp y ) mod p.
-Proof. intros; unfold evalp; rewrite WordByWordMontgomery.eval_submod with (r' := 2 ^ 63); lauto. Qed.
+Lemma eval_sub: forall x y, WordByWordMontgomery.valid bitwidth n p x -> WordByWordMontgomery.valid bitwidth n p y -> (evalp (x -p y)) mod p = ( evalp x - evalp y ) mod p.
+Proof. intros; unfold evalp; rewrite WordByWordMontgomery.eval_submod with (r' := r'); lauto. Qed.
 
-Lemma eval_add: forall x y, WordByWordMontgomery.valid 64 2 p x -> WordByWordMontgomery.valid 64 2 p y -> (evalp (x +p y)) mod p = ( evalp x + evalp y ) mod p.
-Proof. intros; unfold evalp; rewrite WordByWordMontgomery.eval_addmod with (r' := 2 ^ 63); lauto. Qed.
+Lemma eval_add: forall x y, WordByWordMontgomery.valid bitwidth n p x -> WordByWordMontgomery.valid bitwidth n p y -> (evalp (x +p y)) mod p = ( evalp x + evalp y ) mod p.
+Proof. intros; unfold evalp; rewrite WordByWordMontgomery.eval_addmod with (r' := r'); lauto. Qed.
 
-Lemma eval_mul: forall x y, WordByWordMontgomery.valid 64 2 p x -> WordByWordMontgomery.valid 64 2 p y -> (evalp (x *p y)) mod p = ( evalp x * evalp y ) mod p.
-Proof. intros; unfold evalp; rewrite WordByWordMontgomery.eval_mulmod with (r' := 2 ^ 63); lauto. Qed.
+Lemma eval_mul: forall x y, WordByWordMontgomery.valid bitwidth n p x -> WordByWordMontgomery.valid bitwidth n p y -> (evalp (x *p y)) mod p = ( evalp x * evalp y ) mod p.
+Proof. intros; unfold evalp; rewrite WordByWordMontgomery.eval_mulmod with (r' := r'); lauto. Qed.
 
-Lemma eval_sub_mod: forall x y, WordByWordMontgomery.valid 64 2 p x -> WordByWordMontgomery.valid 64 2 p y -> (evalp (x -p y)) mod p = ( evalp x mod p - evalp y mod p ) mod p.
+Lemma eval_sub_mod: forall x y, WordByWordMontgomery.valid bitwidth n p x -> WordByWordMontgomery.valid bitwidth n p y -> (evalp (x -p y)) mod p = ( evalp x mod p - evalp y mod p ) mod p.
 Proof. intros; rewrite eval_sub; try assumption; apply Zminus_mod. Qed.
 
-Lemma eval_add_mod: forall x y, WordByWordMontgomery.valid 64 2 p x -> WordByWordMontgomery.valid 64 2 p y -> (evalp (x +p y)) mod p = ( evalp x mod p + evalp y mod p ) mod p.
+Lemma eval_add_mod: forall x y, WordByWordMontgomery.valid bitwidth n p x -> WordByWordMontgomery.valid bitwidth n p y -> (evalp (x +p y)) mod p = ( evalp x mod p + evalp y mod p ) mod p.
 Proof. intros; rewrite eval_add; try assumption; apply Z.add_mod; unfold p; auto with zarith. Qed.
 
-Lemma eval_mul_mod: forall x y, WordByWordMontgomery.valid 64 2 p x -> WordByWordMontgomery.valid 64 2 p y -> (evalp (x *p y)) mod p = ( evalp x mod p * (evalp y mod p) ) mod p.
+Lemma eval_mul_mod: forall x y, WordByWordMontgomery.valid bitwidth n p x -> WordByWordMontgomery.valid bitwidth n p y -> (evalp (x *p y)) mod p = ( evalp x mod p * (evalp y mod p) ) mod p.
 Proof. intros; rewrite eval_mul; try assumption; apply Z.mul_mod; unfold p; auto with zarith. Qed.
 
 
@@ -192,7 +223,7 @@ Theorem to_montFp2_correct: forall x y, evalFp2 (tomontFp2 (x, y)) = (x, y).
 Proof.
     intros x y; apply injective_projections; [case x | case y];
     intros val Hval; apply zirr; simpl; apply eval_tomont_inv;
-    rewrite Hval; apply Z_mod_lt; unfold p, c, s; simpl; lia.
+    rewrite Hval; apply Z_mod_lt; unfold p; simpl; lia.
 Qed.
 
 (*Reification and subsequent printing to C of field operations.
@@ -234,17 +265,7 @@ Local Existing Instance ToString.C.OutputCAPI.
 Local Instance : static_opt := true.
 Local Instance : internal_static_opt := true.
 Local Instance : emit_primitives_opt := true.
-
-Compute
-     (Pipeline.BoundsPipelineToString
-        "fiat_" "fiat_mulFp2_"
-        false None [1; 64; 128] 64
-        ltac:(let r := Reify (mulFp2r) in
-              exact r)
-              (fun _ _ => [])
-              (Some (repeat (Some r[0~>2^64 - 1]) 2), (Some (repeat (Some r[0~>2^64 - 1]) 2), (Some (repeat (Some r[0~>2^64 - 1]) 2) , (Some (repeat (Some r[0~>2^64 - 1]) 2), tt))))%zrange
-              (Some (repeat (Some r[0~>2^64 - 1]) 2), Some (repeat (Some r[0~>2^64 - 1]) 2))%zrange).
-
+(* 
 Compute
      (Pipeline.BoundsPipelineToString
      "fiat_" "fiat_addFp2_"
@@ -252,8 +273,8 @@ Compute
      ltac:(let r := Reify (addFp2r) in
            exact r)
            (fun _ _ => [])
-           (Some (repeat (Some r[0~>2^64 - 1]) 2), (Some (repeat (Some r[0~>2^64 - 1]) 2), (Some (repeat (Some r[0~>2^64 - 1]) 2) , (Some (repeat (Some r[0~>2^64 - 1]) 2), tt))))%zrange
-           (Some (repeat (Some r[0~>2^64 - 1]) 2), Some (repeat (Some r[0~>2^64 - 1]) 2))%zrange).
+           (Some (repeat (Some r[0~>2^64 - 1]) 6), (Some (repeat (Some r[0~>2^64 - 1]) 6), (Some (repeat (Some r[0~>2^64 - 1]) 6) , (Some (repeat (Some r[0~>2^64 - 1]) 6), tt))))%zrange
+           (Some (repeat (Some r[0~>2^64 - 1]) 6), Some (repeat (Some r[0~>2^64 - 1]) 6))%zrange).
 
 Compute
      (Pipeline.BoundsPipelineToString
@@ -262,8 +283,18 @@ Compute
      ltac:(let r := Reify (subFp2r) in
            exact r)
            (fun _ _ => [])
-           (Some (repeat (Some r[0~>2^64 - 1]) 2), (Some (repeat (Some r[0~>2^64 - 1]) 2), (Some (repeat (Some r[0~>2^64 - 1]) 2) , (Some (repeat (Some r[0~>2^64 - 1]) 2), tt))))%zrange
-           (Some (repeat (Some r[0~>2^64 - 1]) 2), Some (repeat (Some r[0~>2^64 - 1]) 2))%zrange).
+           (Some (repeat (Some r[0~>2^64 - 1]) 6), (Some (repeat (Some r[0~>2^64 - 1]) 6), (Some (repeat (Some r[0~>2^64 - 1]) 6) , (Some (repeat (Some r[0~>2^64 - 1]) 6), tt))))%zrange
+           (Some (repeat (Some r[0~>2^64 - 1]) 6), Some (repeat (Some r[0~>2^64 - 1]) 6))%zrange).
+
+Compute
+     (Pipeline.BoundsPipelineToString
+        "fiat_" "fiat_mulFp2_"
+        false None [1; 64; 128] 64
+        ltac:(let r := Reify (mulFp2r) in
+              exact r)
+              (fun _ _ => [])
+              (Some (repeat (Some r[0~>2^64 - 1]) 6), (Some (repeat (Some r[0~>2^64 - 1]) 6), (Some (repeat (Some r[0~>2^64 - 1]) 6) , (Some (repeat (Some r[0~>2^64 - 1]) 6), tt))))%zrange
+              (Some (repeat (Some r[0~>2^64 - 1]) 6), Some (repeat (Some r[0~>2^64 - 1]) 6))%zrange).
 
 (* The generated code makes calls to the functions; fiat_cmovznz_u64,
    fiat_addcarryx_u64, fiat_subborrowx_u64 and fiat_mulx_u64.
@@ -307,4 +338,4 @@ Compute
             exact r)
              (fun _ _ => [])
              (Some r[0~>2^64-1], (Some r[0~>2^64-1], tt))%zrange
-             (Some r[0~>2^64-1], Some r[0~>2^64-1])%zrange).
+             (Some r[0~>2^64-1], Some r[0~>2^64-1])%zrange). *)
