Examples/BLS12/BLS12Curve.v
@@ -1,0 +1,124 @@
+Require Import Lia.
+Require Import Crypto.Curves.Weierstrass.Projective.
+From Coq Require Import Field.
+From Coqprime Require Import GZnZ.
+Require Import ZArith Znumtheory.
+From Coqprime Require Import Pmod.
+Require Import Theory.FieldsUtil.
+Require Import Theory.RingsUtil.
+Require Import Crypto.Util.Decidable.
+
+Section BLS12Curve1.
+
+    Notation "n 'zmod' p" := (mkznz p (n mod p) (modz p n)) (at level 90).
+
+    Definition u := -0xd201000000010000.
+    Definition p_of_u u := (((u - 1)^2 * (u^4 - u^2 + 1)) / 3) + u.
+    Definition p := Eval compute in (p_of_u u).
+    Hypothesis p_prime : prime p.
+    Definition F := znz p.
+    Definition Feq := @eq F.
+    Definition Fzero := zero p.
+    Definition Fone := one p.
+    Definition Fopp := opp p.
+    Definition Fadd := add p.
+    Definition Fsub := sub p.
+    Definition Fmul := mul p.
+    Definition Finv := inv p.
+    Definition Fdiv := div p.
+    Definition a := Fzero.
+    Definition b := 4 zmod p.
+
+    Add Field Fp : (FZpZ p p_prime).
+
+    Lemma p_ge_3: 3 < p.
+    Proof. unfold p. lia. Qed.   
+
+    Definition field := @std_to_fiatCrypto_field F Fzero Fone Fadd Fmul Fsub Fopp Fdiv Finv (FZpZ p p_prime).
+
+    Definition char_ge_3 := @Char_geq_p p 3 p_ge_3.
+
+
+    Lemma Feq_dec: DecidableRel Feq.
+    Proof.
+        intros. case x as [xval Hx], y as [yval Hy]. destruct (xval =? yval) eqn:case.
+            - rewrite Z.eqb_eq in case. left. apply zirr. auto.
+            - rewrite Z.eqb_neq in case. right. unfold not. intros. inversion H as [H1]. contradiction.
+    Qed.
+
+    Notation "x +p y" := (add p x y) (at level 100).
+    Notation "x *p y" := (mul p x y) (at level 90).
+    Notation "x -p y" := (sub p x y) (at level 100).
+    Notation "x /p y" := (div p x y) (at level 90).
+    Notation "n 'zmod' p" := (mkznz p (n mod p) (modz p n)) (at level 90).
+
+
+    Definition three_b : F := (b +p b +p b).
+    Lemma three_b_correct : (three_b = (b +p b +p b)).
+    Proof. auto. Qed.
+    Check three_b_correct.
+    Local Notation "4" := (Fone +p Fone +p Fone +p Fone).
+    Local Notation "27" := ((4 *p 4) +p 4 +p 4 +p Fone +p Fone +p Fone).
+    Lemma discriminant_nonzero: id(((4 *p a *p a *p a) +p (27 *p b *p b)) <> Fzero).
+    Proof.
+        intros contra; inversion contra.
+    Qed.
+    
+
+    Check @Ring.char_ge F Feq Fzero Fone Fopp Fadd Fsub Fmul.
+
+    Lemma char_ge_21: @Ring.char_ge F Feq Fzero Fone Fopp Fadd Fsub Fmul (21%positive).
+    Proof.
+        pose proof @Char_geq_p p 21; assert (21 < p) by (unfold p; lia); auto.
+    Qed.
+    
+
+
+    Check  @Projective.add F Feq Fzero Fone Fopp Fadd Fsub Fmul Finv Fdiv a b field char_ge_3
+            Feq_dec three_b three_b_correct discriminant_nonzero char_ge_21.
+
+
+
+
+    Definition point := @Projective.point F Feq Fzero Fadd Fmul a b.
+
+    Definition eq (x y : point) := @Projective.eq F Feq Fzero Fadd Fmul a b Feq_dec x y.
+
+    Definition opp (x : point) := @Projective.opp F Feq Fzero Fone Fopp Fadd Fsub Fmul Finv Fdiv a b field Feq_dec x.
+
+    Definition thisP := (0 zmod p, 2 zmod p, 0 zmod p).
+(*
+    Definition point_cond1 X Y Z := (Y *p Y *p Z) = (X *p X *p X +p a *p X *p Z *p Z +p b *p Z *p Z *p Z).
+
+    Check point_cond1.
+
+    Definition point_cond2 Y Z :=
+        Z = Fzero -> Y <> Fzero.
+
+    Definition P_correct P := let '(X, Y, Z) := P in
+        (point_cond1 X Y Z) /\ (point_cond2 Y Z).
+
+    Lemma thisPcorrect: P_correct thisP.
+    Proof.
+        simpl. split.
+            - assert (H: Fzero = (0 zmod p)) by auto. rewrite <- H. auto.
+            - discriminate.
+    Qed.
+*)
+
+    Variable myP : point.
+
+    Program Definition thiseq (P Q : point) : Prop :=
+        (@Projective.eq F Feq Fzero Fadd Fmul a b Feq_dec P Q).
+
+    Program Definition thisopp (P : point) : point :=
+        (@Projective.opp F Feq Fzero Fone Fopp Fadd Fsub Fmul Finv Fdiv a b field Feq_dec P).
+
+
+    Program Definition thisadd (P Q: point) (except : Projective.not_exceptional P Q) : point :=
+        (@Projective.add F Feq Fzero Fone Fopp Fadd Fsub Fmul Finv Fdiv a b field char_ge_3
+        Feq_dec three_b three_b_correct discriminant_nonzero char_ge_21) P Q except.
+
+End BLS12Curve1.
+
+
