Examples/p127/Example127Solinas.v
@@ -1,0 +1,596 @@
+Require Import Crypto.Arithmetic.Core.
+Require Import Crypto.Arithmetic.ModOps.
+Require Import ZArith Znumtheory List.
+Require Import Crypto.Arithmetic.Saturated.
+Require Import Coqprime.Z.Pmod.
+Require Import Lia.
+Require Import Crypto.Arithmetic.Partition.
+Require Import Crypto.Arithmetic.UniformWeight.
+Require Import Crypto.Stringification.IR.
+Require Import Theory.QuadraticFieldExtensions.
+Require Import Coqprime.elliptic.GZnZ.
+
+Require Import Coq.QArith.QArith.
+Require Import Coq.QArith.Qround.
+Require Import Coq.Strings.String.
+Require Import Coq.ZArith.ZArith.
+Require Import Coq.Lists.List.
+Require Import Crypto.Util.ZRange.
+Require Import Rewriter.Language.Language.
+Require Import Crypto.Language.API.
+Require Import Crypto.Stringification.C.
+Require Import Crypto.Arithmetic.Core.
+Require Import Crypto.Arithmetic.ModOps.
+Require Import Crypto.Arithmetic.Primitives.
+Require Import Crypto.BoundsPipeline.
+Import ListNotations.
+Local Open Scope Z_scope. Local Open Scope list_scope.
+Require Import Crypto.PushButtonSynthesis.SaturatedSolinas.
+
+Import
+Language.Compilers
+Stringification.C.Compilers.
+Import Compilers.API.
+
+Import Associational Positional.
+Import ListNotations.
+Import Util.LetIn.
+Import ZUtil.Definitions.
+
+Local Coercion Z.of_nat : nat >-> Z.
+Local Coercion QArith_base.inject_Z : Z >-> Q.
+
+(** ======= these are the changable parameters ====== *)
+Definition s := 2^127.
+Definition c := [(1, 1)].
+Let machine_wordsize := 64.
+Definition p := Eval compute in (s - Associational.eval c).
+(** ================================================= *)
+Let possible_values := [0; 1; 64; 128].
+Definition n := 2%nat.
+Hypothesis n_val: n = Z.to_nat (Qceiling (Z.log2_up s / machine_wordsize)).
+Let m := s - Associational.eval c.
+Let nreductions : nat :=
+  let i := fold_right Z.max 0 (map (fun t => Z.log2 (fst t) / machine_wordsize) c) in
+  Z.to_nat (Qceiling (Z.of_nat n / (Z.of_nat n - i))).
+Let bound := Some r[0 ~> (2^machine_wordsize - 1)]%zrange.
+Let boundsn : list (ZRange.type.option.interp base.type.Z)
+  := repeat bound n.
+Definition w := weight 64 1.
+
+
+Require Import Crypto.Util.ListUtil.
+
+Lemma combine_lemma: forall (A: Type) x' l x n, S (length l) = n -> @combine Z A (map w (seq 0 (n + 1))) (x' :: l ++ [x]) = combine (map w (seq 0 n)) (x' :: l) ++ [(w n, x)].
+Proof.
+    intros A x' l x n Hl. assert (H: seq 0 (n + 1) = (seq 0 n ++ [n])).
+        - assert (n + 1 = S n) by auto with zarith. assert (seq 0 (n + 1) = seq 0 (S n)). auto with zarith. rewrite H0. rewrite seq_S. simpl. auto.
+        - rewrite H. rewrite map_app. simpl. remember (map w (seq 0 n)) as l1. remember (x' :: l) as l2.
+          assert (x' :: l ++ [x] = (x' :: l) ++ [x]). auto. rewrite H0. rewrite combine_snoc. rewrite Heql2. auto.
+          simpl. rewrite Heql1. assert (length (seq 0 n) = n). simpl. apply seq_length. rewrite map_length. rewrite H1. auto.
+Qed.
+
+
+
+Lemma mulmod_rep_compat: forall l x n, length l = n -> Positional.eval w (n + 1) (l ++ [x])
+    = (Positional.eval w n l) +  (w n) * x.
+Proof.
+    intros l x n H. induction l as [|x' l' IHl'].
+        - simpl. simpl in H. rewrite <- H. simpl. unfold eval. unfold to_associational. simpl. unfold Associational.eval. simpl. auto with zarith.
+        - unfold eval. unfold to_associational. simpl. rewrite combine_lemma.
+          rewrite eval_app. assert (Associational.eval [(w n, x)] = w n * x). unfold Associational.eval. simpl. auto with zarith.
+          rewrite H0. auto.
+          simpl in H. auto.
+Qed.
+(*viser at list Z * Z -> list Z korrekt for Rows.mulmod*)
+
+Instance subrelation_eq_impl : subrelation eq Basics.impl.
+congruence.
+Qed.
+
+Instance subrelation_eq_flip_impl : subrelation eq (Basics.flip Basics.impl).
+congruence.
+Qed.
+
+Definition mulp := @Saturated.Rows.mulmod (weight machine_wordsize 1) (2^machine_wordsize) s c 2 nreductions.
+
+Lemma list_len_neq_0: forall (A : Type) (l : list A), 0 < length l -> exists l' x, l = l' ++ [x].
+Proof.
+    intros A l H. induction l as [|x l' IHl'].
+        - simpl in H. discriminate H.
+        - destruct l' eqn:eq.
+            + exists [], x. auto.
+            + assert (0 < length (a :: l)). auto. apply IHl' in H0. inversion H0. inversion H1.
+              exists  (x :: x0). exists x1. rewrite H2. auto.
+Qed.
+
+Definition all_ge_0 l := forall x, In x l -> 0 <= x.
+
+
+
+Lemma weight_ge_0: forall m, 0 <= (w m).
+Proof.
+    intros; unfold w, weight; auto with zarith.
+Qed.
+
+Definition list_prop l := forall m, all_ge_0 l -> length l = m -> 0 <= Positional.eval w m l.
+
+Lemma mulmod_fst_ge_0: forall x, all_ge_0 x -> list_prop x.
+intros. apply (rev_ind list_prop).
+    - unfold list_prop. intros. rewrite eval_nil. auto with zarith.
+    - intros z x' H2 m H3 H4. unfold list_prop. rewrite last_length in H4. rewrite <- H4.
+      rewrite eval_snoc_S; [|reflexivity]. unfold list_prop in H2. apply Z.add_nonneg_nonneg.
+       + apply H2. intros p H'. assert (In p (x' ++ [z])) by (apply in_or_app; auto). apply H3 in H0. auto.
+         auto.
+       + assert (In z (x' ++ [z])) by (apply in_or_app; right; simpl; auto). apply H3 in H0.
+         apply Ztac.mul_le; [apply weight_ge_0 |auto].
+Qed.
+(*
+Lemma mulmod_all_ge_0: forall x y, all_ge_0 x -> all_ge_0 y -> all_ge_0 (fst (mulp x y)).
+Proof.
+    intros. remember (fst (mulp x y)) as l. induction l.
+        - unfold all_ge_0; contradiction.
+        - unfold mulp in Heql. unfold Rows.mulmod in Heql. Check Rows.flatten. unfold Rows.flatten in Heql.
+          unfold Rows.flatten' in Heql.
+Qed.
+
+
+
+
+
+
+
+Lemma mulmod_snd_0: forall x y, (snd (Saturated.Rows.mulmod w 64 s c n nreductions x y)) mod (s - Associational.eval c) = 0.
+Proof.
+    intros x y. destruct (snd (Rows.mulmod w 64 s c n nreductions x y) mod (s - Associational.eval c) =? 0) eqn:eq.
+        - rewrite Z.eqb_eq in eq; auto.
+        - rewrite Z.eqb_neq in eq. remember (snd (Rows.mulmod w 64 s c n nreductions x y) mod (s - Associational.eval c)) as t.
+          assert (0%Z <= t).
+          rewrite Heqt.
+          remember (snd (Rows.mulmod w 64 s c n nreductions x y)) as t'. remember (s - Associational.eval c) as p.
+          assert (H: 0 <= t' mod p < p).
+            + Check t'. Check p. Check Z.mod_pos_bound.
+            apply Z.mod_pos_bound. rewrite Heqp. simpl. auto. auto with zarith.
+            + destruct H. auto.
+            + assert (H': 0 < t). apply Z.le_neq. auto.                
+              assert (forall m, 1 <= m -> t * m >= m). intros m Hm. apply Z.ge_le_iff.
+              rewrite Z.mul_comm. apply Z.le_mul_diag_r. 1, 2: lia.
+              assert ((Positional.eval w n (fst (mulp x y))
+              + w n * (snd (mulp x y))) mod (s - Associational.eval c)
+              = (Positional.eval w n x * Positional.eval w n y) mod (s - Associational.eval c)). apply Saturated.Rows.eval_mulmod.
+              apply wprops. lia. unfold machine_wordsize. lia. unfold s; lia. unfold s, c; simpl; auto with zarith.
+              unfold n. auto. 1, 2: admit. Search Positional.eval.
+
+
+
+          lia. auto with zarith.
+          assert (H: forall x, Positional.eval w n x <= p).
+            + intros. Search Positional.eval. induction x0.
+                * rewrite Positional.eval_nil. unfold p. auto with zarith.
+                * rewrite eval_cons.
+
+
+*)
+
+Definition mulp_sat_gen := @Saturated.Rows.mulmod (weight machine_wordsize 1) (2^machine_wordsize) s c 2 nreductions.
+Definition mulp_sat := @Saturated.Rows.mulmod (weight machine_wordsize 1) (2^machine_wordsize) s c 2 nreductions.
+Definition evalp x := Positional.eval w n x.
+
+Lemma mul_general : mulp_sat_gen = mulp_sat.
+Proof. auto. Qed.
+
+
+(*
+Lemma testlem : forall x y n, n <> 0%nat -> length x = n -> length y = n
+    -> (Positional.eval w n (fst (mulp_sat_gen x y)) + (w n) * (snd (mulp_sat_gen x y))) mod (s - Associational.eval c)
+        = (((Positional.eval w n x) * (Positional.eval w n y) mod (s - Associational.eval c))).
+Proof.
+    intros. unfold mulp_sat_gen. rewrite Saturated.Rows.eval_mulmod. try (unfold s; auto with zarith). 2: unfold machine_wordsize; auto with zarith.
+    2: unfold c; simpl; auto with zarith.
+    About weight_properties. apply wprops. unfold machine_wordsize; auto with zarith.
+Qed.
+
+Definition mulp x y := let (p, p') := mulp_sat x y in
+    p ++ [p'] .
+Definition evalp x := Positional.eval w n x.
+
+Lemma mulp_format: forall x y, mulp x y = (fst (mulp_sat x y)) ++ [snd (mulp_sat x y)].
+Proof. auto. Qed.
+*)
+
+Definition subp x y := Saturated.Rows.sub w n x y.
+
+Definition n1 := 3.
+Definition n2 := 7.
+Definition enc x := Positional.encode w 2 s c x.
+Definition s1 := enc n1.
+Definition s2 := enc n2.
+
+
+(* 
+Lemma mulp_correct: forall x y, (evalp x * evalp y) mod p = evalp (mulp x y) mod p.
+Proof.
+    intros. rewrite mulp_format. unfold evalp. pose proof Saturated.Rows.eval_mulmod. unfold evalp. rewrite <- mul_general. induction n as [|n' IHn'].
+        - rewrite 2!eval0; auto with zarith.
+        - assert (S n' = (n' + 1)%nat). auto with zarith. rewrite H0. rewrite Positional.eval_snoc with (n := n'); auto. rewrite mulmod_rep_compat. *)
+
+
+(* 
+Check Saturated.Rows.mulmod.
+Check Saturated.Rows.flatten'.
+Check ModOps.carry_mulmod.
+
+About Positional.
+
+
+
+Check Positional.encode w 2 s c.
+
+Definition thatx := 2^63 + 1.
+Definition thaty := 2^64.
+
+
+Definition encx x := Positional.encode w 2 s c x.
+Definition thisx := encx thatx.
+Definition thisy := encx thaty.
+
+Eval compute in thisx.
+Eval compute in thisy.
+
+Eval compute in (mulp_sat thisx thisy).
+
+
+Eval compute in (w 2).
+Eval compute in (2^128).
+
+Check flat_map.
+Check Columns.eval.
+
+Lemma test: forall x y, snd (mulp_sat x y) = 0.
+Proof.
+    intros. unfold mulp_sat. Check Rows.mulmod. unfold Rows.mulmod. Check Rows.flatten. unfold Rows.flatten.
+    Check Rows.flatten'. unfold Rows.flatten'. Check fold_right. Search fold_right. remember x as thisx. induction (length x) as [|l' IHl'] eqn:eq.
+    - Search ((length _) = 0).
+Qed.
+
+Local Existing Instances ToString.C.OutputCAPI Pipeline.show_ErrorMessage.
+Local Instance : only_signed_opt := false.
+Local Instance : no_select_opt := false.
+Local Instance : static_opt := true.
+Local Instance : internal_static_opt := true.
+Local Instance : use_mul_for_cmovznz_opt := false.
+Local Instance : emit_primitives_opt := true.
+Local Instance : should_split_mul_opt := false.
+Local Instance : should_split_multiret_opt := false.
+Local Instance : widen_carry_opt := false.
+Local Instance : widen_bytes_opt := true. (* true, because we don't allow byte-sized things anyway, so we should not expect carries to be widened to byte-size when emitting C code *)
+Local Instance : machine_wordsize_opt := machine_wordsize. (* for show *)
+Local Instance : no_select_size_opt := no_select_size_of_no_select machine_wordsize.
+Local Instance : split_mul_to_opt := split_mul_to_of_should_split_mul machine_wordsize possible_values.
+Local Instance : split_multiret_to_opt := split_multiret_to_of_should_split_multiret machine_wordsize possible_values.
+Local Instance : split_mul_to_opt := None.
+Local Instance : split_multiret_to_opt := None.
+Local Instance : unfold_value_barrier_opt := true.
+Local Instance : only_signed_opt := false.
+Local Instance : no_select_size_opt := None.
+Local Existing Instance default_low_level_rewriter_method.
+Local Existing Instance ToString.C.OutputCAPI.
+Local Instance : static_opt := true.
+Local Instance : internal_static_opt := true.
+Local Instance : emit_primitives_opt := true.
+  
+Time Redirect "log" Compute
+      Show.show (* [show] for pretty-printing of the AST without needing lots of imports *)
+      false
+     (Pipeline.BoundsPipelineToString
+        "fiat" "mul"
+        false (* subst01 *)
+        None (* fancy *)
+        possible_values
+        machine_wordsize
+        ltac:( let n := (eval cbv in n) (* needs to be reduced to reify correctly *) in
+        let nreductions := (eval cbv in nreductions) (* needs to be reduced to reify correctly *) in
+        let r := Reify (@Saturated.Rows.mulmod (weight machine_wordsize 1) (2^machine_wordsize) s c n nreductions) in
+        exact r)
+               (fun _ _ => []) (* comment *)
+               (Some boundsn, (Some boundsn, tt))
+               (Some boundsn, Some r[0~>0x1]%zrange (* Should be: Some r[0~>0]%zrange, but bounds analysis is not good enough *) )).
+
+
+
+
+
+(*See https://github.com/mit-plv/fiat-crypto/blob/3f58bfab8d6cb098f0a75d3738e03e939478356c/src/SlowPrimeSynthesisExamples.v#L100-L304
+søg efter "not exactly equal to a weight, we must adjust it t"*)
+
+Require Import Crypto.SlowPrimeSynthesisExamples.
+
+
+
+
+Definition nred := Eval compute in (nreductions machine_wordsize c n). 
+Hypothesis p_prime: prime p.
+Hypothesis p_ge2: 2 < p.
+Hypothesis pmod: p mod 4 =? 3 = true.
+Definition w := ModOps.weight 64 1.
+Notation "n 'zmod' p" := (mkznz p (n mod p) (modz p n)) (at level 90).
+Check QuadraticFieldExtensions.Quad_non_res.
+Lemma quad_res_minus_1: Quad_non_res p = ((-1) zmod p).
+Proof.
+    reflexivity.
+Qed.
+
+Check Rows.mulmod.
+
+
+Eval compute in (Rows.adjust_s w 6 s).
+Eval compute in (2^128).
+
+
+
+About Saturated.Rows.mulmod.
+Check Positional.encode.
+Definition mul127 x y := (Saturated.Rows.mulmod w base s c 2 nred x y).
+Definition eval127' z := (Positional.eval w 2 z).
+Definition enc127 z := Positional.encode w 2 s c z.
+
+Check mul127.
+
+
+
+
+
+
+Local Notation "x *p y" := (mul127 x y) (at level 90).
+
+Require Import Crypto.Util.LetIn.
+Check @ModOps.addmod.
+
+Definition add127 x y : list Z := ModOps.addmod.
+
+
+Eval compute in ModOps.weight 64 1 2.
+Eval compute in (2^128).
+
+Definition mulFp2 := fun x y => let '(x1, x2) := x in
+    let '(y1, y2) := y in
+    dlet v0 := (x1) *p (y1) in
+        dlet v1 := (x2) *p (y2) in
+            (
+                v0 -p v1,
+                ((((x1) +p (x2)) *p ((y1) +p (y2))) -p v0) -p v1
+            ).
+
+Definition  mulFp2r x1 x2 y1 y2 :=
+        dlet v0 := (x1) *p (y1) in 
+        dlet v1 := (x2) *p (y2) in
+            (
+                v0 -p v1,
+                dlet f1 := x1 +p x2 in
+                    dlet f2 := y1 +p y2 in
+                        dlet v2 := f1 *p f2 in
+                            dlet v3 := v2 -p v0 in
+                                v3 -p v1
+            ).
+
+
+Definition mulFp2reif (x11 x12 x21 x22 y11 y12 y21 y22 : Z) := let '(z1, z2) := (mulFp2 ([x11; x12], [x21; x22]) ([y11; y12], [y21; y22])) in
+    [nth_default 0 z1 0; nth_default 1 z1 0; nth_default 0 z2 0; nth_default 1 z2 0].
+(*
+Definition mulFp2r (x1 x2 y1 y2 : list Z) := mulFp2 (x1, x2) (y1, y2).
+*)
+Definition hej (l1 l2 l3 l4: list Z) : list Z :=
+    l1 +p l2 +p l3.
+
+Definition hej2 x1 x2 y1 y2 :=
+    (dlet v0 := (x1 +p y1) in (
+            dlet v1 := (x2 +p y2) in (
+                x1,
+                x2
+            )
+        )
+    ).
+
+Definition to_montgomeryFp2 x := (tomont127 (val p (fst x)), tomont127 (val p (snd x))).
+
+
+Definition eval_Fp2 x :=
+    (
+        eval127(fst x) zmod p,
+        eval127(snd x) zmod p
+    ).
+
+(*testing*)
+
+Definition z1 := (543254938987987935443 zmod p, 5433 zmod p).
+Definition z2 := (65433 zmod p, 2457 zmod p).
+Definition mon1 := to_montgomeryFp2 z1.
+Definition mon2 := to_montgomeryFp2 z2.
+Definition eval1 := eval_Fp2 mon1.
+Definition eval2 := eval_Fp2 mon2.
+
+Definition prod := mulFp2r (fst mon1) (snd mon1) (fst mon2) (snd mon2).
+Definition prodeval := eval_Fp2 prod.
+
+
+(*Eval compute in (elem1).*)
+Eval compute in (mon1).
+Eval compute in (mon2).
+
+Eval compute in prod.
+Eval compute in prodeval.
+Definition x1 := [2303232; 9223605965625171200].
+Definition x2 := [18446325046823417597; 9223138782394246399].
+Eval compute in eval_Fp2 (x1, x2).
+
+Eval compute in (2^64).
+
+Eval compute in 18446465859655129087.
+
+Definition out0 := .
+
+
+
+Time Redirect "log" Compute
+     (Pipeline.BoundsPipelineToString
+        "fiat_" "fial_mulFp2_"
+        false None [64; 128] 64
+        ltac:(let r := Reify (mulFp2r) in
+              exact r)
+              (fun _ _ => [])
+              (Some (repeat (Some r[0~>2^64 - 1]) 2), (Some (repeat (Some r[0~>2^64 - 1]) 2), (Some (repeat (Some r[0~>2^64 - 1]) 2) , (Some (repeat (Some r[0~>2^64 - 1]) 2), tt))))%zrange
+              (Some (repeat (Some r[0~>2^64 - 1]) 2), Some (repeat (Some r[0~>2^64 - 1]) 2))%zrange).
+
+
+
+
+
+Lemma eval_correct: forall x, x = ((eval127 (tomont127 (val p x))) zmod p).
+Proof.
+    intros x. case x. simpl. intros val inZnZ. apply zirr. unfold eval127, tomont127. Check WordByWordMontgomery.eval_encodemod.
+    rewrite WordByWordMontgomery.eval_encodemod with (r' := 2 ^63); try auto; unfold p, c, s; simpl; unfold Z.pow_pos; simpl; try lia.
+    rewrite inZnZ. unfold p, c, s; simpl. apply Z_mod_lt. lia.
+Qed.
+
+
+Lemma eval_compat: forall x n, Positional.eval w n x = @WordByWordMontgomery.eval 64 n x.
+Proof. auto. Qed.
+
+Lemma eval_encode: forall x n, n <> 0%nat -> Positional.eval w n (Positional.encode w n s c x) mod p = x mod p.
+Proof.
+    intros. apply Positional.eval_encode; (unfold s, c, p; auto with zarith; try lia).
+    - intros. unfold w, uweight. assert (0 < weight 64 1 i). apply weight_positive, wprops; lia. lia.
+    - simpl; lia.
+    - intros. unfold w, uweight. assert (0 < (weight 64 1 (S i)) / (weight 64 1 i)). apply weight_divides, wprops; lia. lia.
+Qed.
+
+
+Eval compute in (uweight 64 1).
+
+Theorem eval_tomont_inv: forall val, 0 <= val < p -> eval127 (tomont127 val) mod p = val.
+Proof.
+    intros val H; unfold eval127, tomont127; rewrite WordByWordMontgomery.eval_encodemod with (r' := 2 ^ 63);
+    (unfold p, s, c; simpl; unfold Z.pow_pos; simpl; auto with zarith; lia).
+Qed.
+
+
+Theorem to_montFp2_correct: forall x y, eval_Fp2 (to_montgomeryFp2 (x, y)) = (x, y).
+Proof.
+    intros; unfold eval_Fp2; apply injective_projections; [case x | case y];
+    intros val Hval; apply zirr; simpl; apply eval_tomont_inv;
+    rewrite Hval; apply Z_mod_lt; unfold p, c, s; simpl; lia.
+Qed.
+
+Definition tomontFp2:= fun x => (tomont127 (val p (fst x)), tomont127 (val p (snd x))).
+Definition evalFp2:= fun x => (eval127 (fst x) zmod p, eval127 (snd x) zmod p).
+
+Local Ltac thisauto := unfold p, c, s; simpl; unfold Z.pow_pos; simpl; auto with zarith.
+
+(*SKRIV DETTE RENT!!!!!*)
+Theorem add127_correct: forall x y, (eval127(tomont127 (val p x) +p tomont127 (val p y)) zmod p) = add p x y.
+Proof.
+    intros x y. unfold add127. unfold add. simpl. apply zirr. unfold eval127.
+    rewrite WordByWordMontgomery.eval_addmod with (r' := 2 ^ 63); [|thisauto|thisauto|thisauto|thisauto|thisauto|thisauto| | ].
+        - unfold tomont127. rewrite PullPush.Z.add_mod_full.
+        assert  (forall z, (@WordByWordMontgomery.eval 64 2
+                (WordByWordMontgomery.from_montgomerymod 64 2 p 1
+                (WordByWordMontgomery.encodemod 64 2 p 1 z)) mod p)
+           = eval127 (tomont127 z) mod p); [auto|].
+        do 2 rewrite H.
+        repeat rewrite eval_tomont_inv; try reflexivity;
+        [destruct y| destruct x]; simpl; rewrite inZnZ; apply Z_mod_lt; thisauto.
+        - pose proof WordByWordMontgomery.encodemod_correct 64 2 p (2 ^ 63) 1. apply H;
+          try ( unfold p, c, s; simpl; unfold Z.pow_pos; simpl; auto with zarith; lia).
+          destruct x. simpl. rewrite inZnZ. apply Z_mod_lt. unfold p, c, s; simpl; lia.
+        - unfold tomont127.
+          pose proof WordByWordMontgomery.encodemod_correct 64 2 p (2 ^ 63) 1. apply H;
+          try ( unfold p, c, s; simpl; unfold Z.pow_pos; simpl; auto with zarith; lia).
+          destruct y. simpl. rewrite inZnZ. apply Z_mod_lt. unfold p, c, s; simpl; lia.
+Qed.
+
+Theorem add_correct: forall x y, evalFp2 (addFp2 (tomontFp2 x) (tomontFp2 y)) = addp2 p x y.
+Proof.
+    intros x y. unfold evalFp2, tomontFp2. simpl. unfold addp2. apply injective_projections; (simpl; rewrite add127_correct; reflexivity).
+Qed.
+
+
+Theorem mul127_correct: forall x y, (eval127 (tomont127 (val p x) *p tomont127 (val p y)) zmod p) = mul p x y.
+Proof.
+    intros x y. unfold mul127. unfold mul. simpl. apply zirr. unfold eval127.
+    rewrite WordByWordMontgomery.eval_mulmod with (r' := 2 ^ 63); [|thisauto|thisauto|thisauto|thisauto|thisauto|thisauto| | ].
+        - unfold tomont127. rewrite Z.mul_mod; [| unfold p, c, s; simpl; auto with zarith].
+        assert  (forall z, (@WordByWordMontgomery.eval 64 2
+                (WordByWordMontgomery.from_montgomerymod 64 2 p 1
+                (WordByWordMontgomery.encodemod 64 2 p 1 z)) mod p)
+           = eval127 (tomont127 z) mod p); [auto|].
+        do 2 rewrite H.
+        repeat rewrite eval_tomont_inv; try reflexivity;
+        [destruct y| destruct x]; simpl; rewrite inZnZ; apply Z_mod_lt; thisauto.
+        - pose proof WordByWordMontgomery.encodemod_correct 64 2 p (2 ^ 63) 1. apply H;
+          try ( unfold p, c, s; simpl; unfold Z.pow_pos; simpl; auto with zarith; lia).
+          destruct x. simpl. rewrite inZnZ. apply Z_mod_lt. unfold p, c, s; simpl; lia.
+        - unfold tomont127.
+          pose proof WordByWordMontgomery.encodemod_correct 64 2 p (2 ^ 63) 1. apply H;
+          try ( unfold p, c, s; simpl; unfold Z.pow_pos; simpl; auto with zarith; lia).
+          destruct y. simpl. rewrite inZnZ. apply Z_mod_lt. unfold p, c, s; simpl; lia.
+Qed.
+
+Theorem mul127_corr: forall x y, (eval127((tomont127 (val p x)) *p (tomont127 (val p y))) zmod p) = (eval127 (tomont127 (val p x)) zmod p).
+Proof.
+    unfold eval127, tomont127. Abort.
+
+Add Field fp : (FZpZ p p_prime).
+Theorem mul_correct: forall x y, evalFp2 (mulFp2 (tomontFp2 x) (tomontFp2 y)) = mulp2 p x y.
+Proof.
+    intros x y. unfold mulFp2, mulp2. simpl. apply Fp2irr.
+    simpl. apply zirr. unfold eval127. rewrite WordByWordMontgomery.eval_submod with (r' := 2 ^ 63).
+        - Search (((?n1 mod ?n3) * (?n2 mod ?n3)) mod ?n3 ). rewrite Zminus_mod.
+          repeat rewrite WordByWordMontgomery.eval_mulmod with (r' := 2^63).
+            + unfold tomont127. rewrite Z.mul_mod. rewrite WordByWordMontgomery.eval_encodemod with (r' := 2 ^ 63).
+              rewrite WordByWordMontgomery.eval_encodemod with (r' := 2 ^ 63).
+              pose proof (Z.mul_mod (@WordByWordMontgomery.eval 64 2
+              (WordByWordMontgomery.from_montgomerymod 64
+                 2 p 1
+                 (WordByWordMontgomery.encodemod 64 2 p 1
+                    (val p (snd x))))) ( @WordByWordMontgomery.eval 64 2
+                    (WordByWordMontgomery.from_montgomerymod 64
+                       2 p 1
+                       (WordByWordMontgomery.encodemod 64 2 p 1
+                          (val p (snd y))))) p). rewrite H.
+                          rewrite WordByWordMontgomery.eval_encodemod with (r' := 2 ^ 63).
+              rewrite WordByWordMontgomery.eval_encodemod with (r' := 2 ^ 63).
+              rewrite <- Z.mul_mod. rewrite <- Z.mul_mod. rewrite <- Zminus_mod. rewrite quad_res_minus_1.
+              ring_simplify. unfold mul. assert ((-1 zmod p) = opp p (1 zmod p)). auto. simpl. simpl. ring. 
+    unfold tomont127. rewrite mul_correct. 
+Qed.
+
+
+Local Instance : split_mul_to_opt := None.
+Local Instance : split_multiret_to_opt := None.
+Local Instance : unfold_value_barrier_opt := true.
+Local Instance : only_signed_opt := false.
+Local Instance : no_select_size_opt := None.
+Local Existing Instance default_low_level_rewriter_method.
+
+
+Local Existing Instance ToString.C.OutputCAPI.
+Local Instance : static_opt := true.
+Local Instance : internal_static_opt := true.
+Local Instance : emit_primitives_opt := true.
+
+
+(*
+Lemma s_nz: s <> 0.
+Proof. unfold s; auto with zarith. Qed.
+
+Lemma m_nz: s - Associational.eval c <> 0.
+Proof. unfold s, c; simpl; auto with zarith. Qed.
+
+Definition force_carry l := (Positional.chained_carries w 3 s c l [0%nat;1%nat;2%nat]).
+
+Definition m' := 1.
+Definition r := 2 ^ 64.
+
+Lemma m'_correct : (p * m') mod r = (-1) mod r.
+Proof. auto with zarith. Qed.
+*) *)
