Rupicola/test/laddertest.v
@@ -1,0 +1,94 @@
+Require Import Rupicola.Lib.Api.
+Require Import Rupicola.Lib.SepLocals.
+Require Import Rupicola.Lib.ControlFlow.CondSwap.
+Require Import Rupicola.Lib.ControlFlow.DownTo.
+Require Import Crypto.Arithmetic.PrimeFieldTheorems.
+Require Import Crypto.Bedrock.Field.Interface.Compilation.
+Require Import Crypto.Bedrock.Group.Point.
+Require Import Crypto.Bedrock.Group.ScalarMult.LadderStep.
+Require Import Crypto.Bedrock.Specs.Field.
+Require Import Crypto.Bedrock.Specs.ScalarField.
+Require Import Crypto.Util.NumTheoryUtil.
+Require Import Crypto.Bedrock.Group.ScalarMult.MontgomeryLadder.
+Require Import bedrock2.Semantics.
+Require Import bedrock2.ToCString.
+Require Import bedrock2.NotationsCustomEntry.
+Require Import bedrock2.NotationsInConstr.
+Require Import Crypto.Spec.ModularArithmetic.
+Require Import Coqprime.elliptic.GZnZ.
+
+
+Coercion expr.var : string >-> Syntax.expr.
+Unset Printing Coercions.
+Local Open Scope bedrock_expr.
+Local Open Scope Z_scope.
+Local Open Scope F_scope.
+
+Require Import bedrock2.BasicC64Semantics.
+
+
+Print FieldParameters.
+Definition thism : positive := 4002409555221667393417789825735904156556882819939007885332058136124031650490837864442687629129015664037894272559787.
+Definition a : Z := 23223.
+Definition toF n := (F.of_Z thism n).
+
+
+Instance field_parameters : FieldParameters :=
+{
+    M_pos := thism;
+    a24 := toF a;
+    mul := "mul";
+    add := "add";
+    sub := "sub";
+    square := "square";
+    scmula24 := "scmula24";
+    inv := "inv";
+    from_bytes := "from_bytes";
+    to_bytes := "to_bytes";
+    felem_copy := "felem_copy";
+    felem_small_literal := "felem_small_literal"
+}.
+
+Hypothesis m_prime: Znumtheory.prime (Z.pos M_pos).
+
+Instance field_parameters_ok : FieldParameters_ok :=
+{
+    M_prime := m_prime
+}.
+
+Check mem.
+Instance field_representation : FieldRepresentation :=
+{
+    felem := Z;
+    feval := toF;
+    feval_bytes l := toF 10;
+    felem_size_in_bytes := 48;
+    FElem (w : word) (f : Z) (m : mem) := True; 
+    bounds := Z; 
+    bounded_by b f := False;
+    loose_bounds := 100;
+    tight_bounds := 100
+    }.
+
+    About Placeholder.
+    Check Placeholder.
+Instance field_representation_ok : FieldRepresentation_ok.
+Proof.
+    constructor; try auto.
+        - intros. split; intros.
+            + exists (12). simpl. auto.
+            + inversion H. simpl in H0. unfold Placeholder.
+
+Definition bedrock_func : Type :=
+    string * (list string * list string * cmd).
+
+    Definition mont_ladder : bedrock_func :=
+        ("mont_ladder",
+         (["arg1"; "arg2"; "arg3"],
+          ["out1"; "out2"],
+          montladder_body)).
+
+Print montladder_body.
+Check montladder_body.
+Check c_func.
+Check c_module.
